\section{Solutions to Chapter 4: Independence}
\label{sec:solutions-chapter-4}

\setcounter{Lcount}{0}
\begin{list}{4.6.\arabic{Lcount}}{\usecounter{Lcount}}
\item
  \[
    P\left(\bigcup\limits_{i=1}^nB_i\right)
    = 1 - P\left(\bigcap\limits_{i = 1}^nB_i^c\right)
    = 1 - \prod\limits_{i = 1}^n P\left(B_i^c\right)
    = 1 - \prod\limits_{i = 1}^n\left(1 - P\left(B_i\right)\right)
  \]
  
\item {\color{red}I guess the answer is $2^n$. But a proof is needed.}
  
\item
  \[
    P\left(\bigcap\limits_{n = 1}^\infty A_n\right)
    = P\left(\underset{m\rightarrow\infty}{\mathrm{lim}}\bigcap\limits_{n = 1}^m A_n\right)
    = \underset{m\rightarrow\infty}{\mathrm{lim}}P\left(\bigcap\limits_{n = 1}^mA_n\right)
    = \underset{m\rightarrow\infty}{\mathrm{lim}}\prod\limits_{n=1}^mP\left(A_n\right)
    = \prod\limits_{n=1}^\infty P\left(A_n\right)
  \]
  The second equation follows the fact that probability measure $P$ is continuous on monotone sequence $\left\{\bigcap\limits_{n=1}^mA_n,\;m\geq1\right\}$.
\end{list}

\clearpage{}

%%% Local Variables:
%%% mode: latex
%%% TeX-master: "../Solutions_A_Probability_Path"
%%% End:
